\textbf{Problem Set }

\vspce

\begin{enumerate}[label = \Alph*. ]
%begin{multicols}{2}

\item \phantom{n}  %Find the indicated sum of the following geometric series.   
  
\begin{enumerate}[label = \arabic*. ]

	\item %\hspce% $9+6+4+\ldots S_7$
$a_1=9$, $S_{7}=? $, $n=7$,\\
$r=6 \div 9=\displaystyle \frac{2}{3} $\\
$\displaystyle S_{n} = \frac{a_1(1-r^n)}{1-r}$\\
$\displaystyle S_{7} = \frac{9\left[ 1-\left(  \frac{2}{3}\right)^7\right] }{1- \frac{2}{3} }$\\
$\displaystyle S_{7} = \frac{9\left( 1- \frac{128}{2187} \right) }{ \frac{1}{3} }$\\
$\displaystyle S_{7} = 9\left(  \frac{2059}{2187} \right)(3)$\\
$\displaystyle S_{7} = \displaystyle \frac{2059}{81} $

	\item %\hspce $2+8+32+\ldots S_{9}$
	$a_1=2$, $S_{9}=?$, $n=9$,\\
$r=8 \div 2=4 $\\
$\displaystyle S_{n} = \frac{a_1(1-r^n)}{1-r}$\\
$\displaystyle S_{9} = \frac{2(1-4^9)}{1-4}$\\
$\displaystyle S_{9} = \frac{2(1-262,144)}{-3}$\\
$\displaystyle S_{9} = \frac{2(-262,143)}{-3}$\\
$\displaystyle S_{9} = \frac{-524,284}{-3}$\\
$S_{9} =174,762$

	\item% \hspce $3+3\sqrt{3}+9+\ldots S_{9}$
		$a_1=3$, $S_{9}=?$, $n=9$,\\
$r=3\sqrt{3} \div 3= \sqrt{3}$\\
$\displaystyle S_{n} = \frac{a_1(1-r^n)}{1-r}$\\
$\displaystyle S_{9} = \frac{3(1-(\sqrt{3})^9)}{1-\sqrt{3}}$\\
$\displaystyle S_{9} = \frac{3(1-81\sqrt{3}}{1-\sqrt{3}}$\\
$\displaystyle S_{9} = \frac{3-243\sqrt{3}}{1-\sqrt{3}}$\\
$\displaystyle S_{9} = \frac{3-243\sqrt{3}}{1-\sqrt{3}}\cdot \displaystyle \frac{1+\sqrt{3}}{1+\sqrt{3}} $\\
$\displaystyle S_{9} = \frac{-726-240 \sqrt{3}}{1-3} $\\
$\displaystyle S_{9} = \frac{-726-240 \sqrt{3}}{-2} $\\
$\displaystyle S_{9} = 363+120 \sqrt{3} $\\

	\item %\hspce $1+(-2)+4+(-8)\ldots S_8$
		$a_1=1$, $S_{8}=?$, $n=8$,\\
$r= -2\div 1= -2$\\
$\displaystyle S_{n} = \frac{a_1(1-r^n)}{1-r}$\\
$\displaystyle S_{8} = \frac{1(1-(-2)^8)}{1-(-2)}$\\
$\displaystyle S_{8} = \frac{1-256}{3}$\\
$\displaystyle S_{8} = \frac{-255}{3}$\\
$ S_{8} = -85$

	\item %\hspce $(-2)+6+(-18)+\ldots S_6$ 
		$a_1=-2$, $S_{6}=?$, $n=6$,\\
$r= 6\div (-2)= -3$\\
$\displaystyle S_{n} = \frac{a_1(1-r^n)}{1-r}$\\
$\displaystyle S_{6} = \frac{(-2)(1-(-3)^6)}{1-(-3)}$\\
$\displaystyle S_{6} = \frac{(-2)(1-729)}{4}$\\
$\displaystyle S_{6} = \frac{(-2)(-728)}{4}$\\
$ S_{6} =364$\\

%%end{multicols} 

\end{enumerate}

\vspce

\item \phantom{b} %Find the sum of the first $n$ terms of the related geometric series. 

\begin{enumerate}[label = \arabic*. ]

%begin{multicols}{2}

\item %\hspce $\displaystyle a_1=\frac{1}{2}; r=4; n=6 $
$ S_{n} = \displaystyle\frac{a_1(1-r^n)}{1-r}$\\
$ S_{6} = \displaystyle\frac{\frac{1}{2}(1-4^6)}{1-4}$\\
$ S_{6} = \displaystyle\frac{\frac{1}{2}(1-4096)}{-3}$\\
$ S_{6} = \displaystyle\frac{\frac{1}{2}(-4095)}{-3}$\\
$ S_{6} = \displaystyle\frac{1365}{2}$\\

\item% \hspce %$\displaystyle a_1=13; r=4; n=7 $ 
$ S_{n} = \displaystyle\frac{a_1(1-r^n)}{1-r}$\\
$ S_{7} = \displaystyle\frac{13(1-4^7)}{1-4}$\\
$ S_{7} = \displaystyle\frac{13(1-16384)}{-3}$\\
$ S_{7} = \displaystyle\frac{13(-16383)}{-3}$\\
$ S_{7} = 70,993$

\item %\hspce $\displaystyle a_1=318; \hspce r=\frac{1}{2};\hspce n=7 $
$ S_{n} = \displaystyle\frac{a_1(1-r^n)}{1-r}$\\
$ S_{7} = \displaystyle\frac{318\left[ 1-\left(\frac{1}{2} \right) ^7\right] }{1-\frac{1}{2}}$\\
$ S_{7} = \displaystyle\frac{318\left[ 1-\left(\frac{1}{128} \right)\right] }{\frac{1}{2}}$\\
$ S_{7} = \displaystyle\frac{318\left[ 1-\left(\frac{1}{128} \right)\right] }{\frac{1}{2}}$\\
$ S_{7} = \displaystyle\frac{318\left(\frac{127}{128} \right) }{\frac{1}{2}}$\\
$ S_{7} =\displaystyle \frac{20193}{32} $

\item %\hspce $\displaystyle a_1=168;\hspce r=\frac{3}{4};\hspce n=8 $
$ S_{n} = \displaystyle\frac{a_1(1-r^n)}{1-r}$\\
$ S_{8} = \displaystyle\frac{168\left[1-\left(\frac{3}{4} \right) ^8\right]}{1-\frac{3}{4}}$\\

$ S_{8} = \displaystyle\frac{168\left[1-\left(\frac{6561}{65536} \right)\right]}{\frac{1}{4}}$\\
$ S_{8} = \displaystyle\frac{168\left(\frac{58975}{65536} \right)}{\frac{1}{4}}$\\

$ S_{8} = \displaystyle\frac{1238475}{2048}$

\item %\hspce $\displaystyle a_1=4;\hspce r=-5; \hspce n=8 $
$ S_{n} = \displaystyle\frac{a_1(1-r^n)}{1-r}$\\
$ S_{8} = \displaystyle\frac{4(1-(-5)^8)}{1-(-5)}$\\
$ S_{8} = \displaystyle\frac{4(1-390625)}{6}$\\
$ S_{8} = \displaystyle\frac{4(-390624)}{6}$\\
$ S_{8} =260416$


%
\end{enumerate}
%end{multicols} 
\end{enumerate}