\textbf{Problem Set}

\vspce


\begin{enumerate} 


\begin{multicols}{2}

\item \hspce $x^{2} + 4x - 21 $\\
$= \left(x - 3\right) \left(x + 7\right)$

\item \hspce $x^{2} - 5x - 14$\\
$= \left(x - 7\right) \left(x + 2\right)$

\item \hspce $2a^{3} + 20a^{2} + 48a	$\\
$= 2 a \left(a + 4\right) \left(a + 6\right)$

\item \hspce $m^{2} + m - 12$\\
$= \left(m - 3\right) \left(m + 4\right)$

\item \hspce $a^{2} - 8a - 48$\\
$= \left(a - 12\right) \left(a + 4\right)$


\item \hspce $3 m^{2} + 6 m n - 45 n^{2} $\\
$= 3 \left(m - 3 n\right) \left(m + 5 n\right)$

\item \hspce $2 b^{3} + 10 b^{2} c - 28 b c^{2}$\\
$= 2b(b+7c)(b-2c)$

\item \hspce $c^{2} - 11 c d + 24 d^{2}$\\
$= (c-8d) (c-3d)$


\item \hspce $5 m^{3} - 20 m^{2} + 15 m$\\
$= 5m(m-1)(m-3)$

\item \hspce $4 a^{2} + 24 a - 64$\\
$= 4(a+8)(a-2)$

\end{multicols} 
 
\end{enumerate}