\begin{center}
\textbf{Quiz \#2}
\end{center} 

\begin{enumerate}[label = \Alph*. ]
\begin{multicols}{2}

%A
\item \phantom{a}
\begin{enumerate}[label = \arabic*. ]
%1
\item $13.8$ and $15.6$ \\
$A. M. = \displaystyle \frac{13.8 + 15.6}{2} $\\
$A. M. =14.7$

%2
\item $4-7\sqrt{7} $ and $2+3\sqrt{7} $\\
$A. M. = \displaystyle \frac{4-7\sqrt{7} + 2+3\sqrt{7}}{2} $\\
$A. M. =3-2\sqrt{7}$

%3
\item $2x+3y$ and $x-5y$\\
$A. M. = \displaystyle \frac{(2x+3y)  + (x-5y) }{2} $\\
$A. M. =\displaystyle \frac{3x-2y}{2}$\\

\end{enumerate}   


%B
\item \phantom{a} 
\begin{enumerate}[label = \arabic*. ]
%1
\item %\#1
$a_1=2$\\
$a_2=2+5=7$\\
$a_3=7+5=12$\\
$a_4=12+5=17$\\
$a_5=22$\\
$d=\displaystyle \frac{a_{n}-a_{k}}{n-k}$\\
$d=\displaystyle \frac{a_{5}-a_{1}}{5-1}$\\
$d=\displaystyle \frac{22-2}{4}$\\
$d=5$

%2
\item %\#8
$a_1=24$\\
$a_2=24+(-7.2)=16.8$\\
$a_3=16.8+(-7.2)=9.6$\\
$a_4=9.6+(-7.2)=2.4$\\
$a_5=2.4+(-7.2)=-4.8$\\
$a_6=-12$\\
$d=\displaystyle \frac{a_{n}-a_{k}}{n-k}$\\
$d=\displaystyle \frac{a_{6}-a_{1}}{6-1}$\\
$d=\displaystyle \frac{-12-24}{5}$\\
$d=-7.2$

%3
\item %\#10
$a_1=2\sqrt{5}$\\
$a_2=2\sqrt{5}+4\sqrt{5}=6\sqrt{5}$\\
$a_3=6\sqrt{5}+4\sqrt{5}=10\sqrt{5}$\\
$a_4=14\sqrt{5}$\\
$d=\displaystyle \frac{a_{n}-a_{k}}{n-k}$\\
$d=\displaystyle \frac{a_{4}-a_{1}}{4-1}$\\
$d=\displaystyle \frac{14\sqrt{5}-2\sqrt{5}}{3}$\\
$d=4\sqrt{5}$
\end{enumerate}   

%C
\item \phantom{a} 
\begin{enumerate}[label = \arabic*. ]
%1
\item %\#4
$a_1=31$\\
$a_2=31+18=49$\\
$a_3=49+18=67$\\
$a_4=85$\\
$d=\displaystyle \frac{a_{n}-a_{k}}{n-k}$\\
$d=\displaystyle \frac{a_{4}-a_{1}}{4-1}$\\
$d=\displaystyle \frac{85-31}{3}$\\
$d=18$

%2
\item %\#10
$a_1=6-8=-2$\\
$a_2=6$\\
$a_3=6+8=14$\\
$a_4=14+8=22$\\
$a_5=30$\\
$d=\displaystyle \frac{a_{n}-a_{k}}{n-k}$\\
$d=\displaystyle \frac{a_{5}-a_{2}}{5-2}$\\
$d=\displaystyle \frac{30-6}{3}$\\
$d=8$

\item %\#13
$A. M. = \displaystyle \frac{x-10\sqrt{3} + x+10\sqrt{3}}{2} $\\
$A. M. =x$

\item %\#14
$a_1=-3 \sqrt{3} $\\
$a_2=-3 \sqrt{3}+3\sqrt{3}=0$\\
$a_3=0+3\sqrt{3}=3\sqrt{3} $\\
$a_4=3\sqrt{3} +3\sqrt{3}=6\sqrt{3} $\\
$a_5=6\sqrt{3}+3\sqrt{3}=9\sqrt{3}$\\
$a_6=9\sqrt{3}+3\sqrt{3}=12\sqrt{3}$\\
$a_7=15 \sqrt{3} $\\
$d=\displaystyle \frac{a_{n}-a_{k}}{n-k}$\\
$d=\displaystyle \frac{a_{7}-a_{1}}{7-1}$\\
$d=\displaystyle \frac{15 \sqrt{3} -(-3 \sqrt{3}) }{6}$\\
$d=3\sqrt{3} $
\end{enumerate}   

\end{multicols} 
\end{enumerate}  