\textbf{Problem Set}

\ 

%Perform the indicated  operation. 
%\ 

\begin{enumerate}[label = \arabic*. ]
%%begin{multicols}{2}

\item \hspce% $\displaystyle \frac{6}{3a-9} - \frac{3}{3a-9}$
$\displaystyle \frac{6-3}{3a-9}$\\
$=\displaystyle \frac{3}{3a-9}$\\
$=\displaystyle \frac{3}{3(a-3)}$\\
$=\dfrac{1}{a - 3} $
\item \hspce% $\displaystyle \frac{x^{2}-3x-7}{x^{2}-9}+\frac{x^{2}-2x+4}{x^{2}-9}$
%$\displaystyle \frac{x^{2}-3x-7+x^{2}-2x+4}{x^{2}-9}$\\
$\displaystyle \frac{x^{2}-3x-7+x^{2}-2x+4}{x^{2}-9}$\\
$=\displaystyle \frac{2 x^{2} - 5 x - 3}{x^{2}-9}$\\
$=\displaystyle \frac{\left(x - 3\right) \left(2 x + 1\right)}{\left(x - 3\right) \left(x + 3\right)}$\\
$=\dfrac{2 x + 1}{x + 3}$

\item \hspce% $\displaystyle \frac{7}{3x-6}-\frac{4}{3x-6}$
$\displaystyle \frac{7-4}{3x-6}$\\
$=\displaystyle \frac{3}{3x-6}$\\
$=\displaystyle \frac{3}{3(x-2)}$\\
$=\dfrac{1}{x - 2}$
\item \hspce% $\displaystyle \frac{x^{2}+2x+2}{x^{2}-4x+4} - \frac{2x+6}{x^{2}-4x+4}$

$=\dfrac{x + 2}{x - 2}$
\item \hspce% $\displaystyle \frac{x-2}{x-4} - \frac{2}{x-4}$

$=1$
%%end{multicols}
\end{enumerate}