\textbf{Problem Set}

\vspce


\begin{enumerate} 
%

\item \hspce $27x^{3} - 64y^{3}z^{6}$\\
$= (3 x)^3 - (4 y z^{2})^3$\\
$= \left(3 x - 4 y z^{2}\right) \left(9 x^{2} + 12 x y z^{2} + 16 y^{2} z^{4}\right)$

\item \hspce $8x^{3} + 125$\\
$= (2 x)^3 + (5)^3$\\
$= \left(2 x + 5\right) \left(4 x^{2} - 10 x + 25\right)$

\item \hspce $64a^{3} - 8b^{9}c^{3}$\\
$=8(8a^{3} - b^{9}c^{3}) $\\
$= 8[(2 a)^3 - ( b^{3} c)^3]$\\
$= 8 \left(2 a - b^{3} c\right) \left(4 a^{2} + 2 a b^{3} c + b^{6} c^{2}\right)$

\item \hspce $27m^{3} + 125n^{3}$\\
$= (3 m )^3 + (5 n)^3$\\
$= \left(3 m + 5 n\right) \left(9 m^{2} - 15 m n + 25 n^{2}\right)$

\item \hspce $64a^{3} + 27$\\
$= (4 a)^3 + (3)^3$\\
$= \left(4 a + 3\right) \left(16 a^{2} - 12 a + 9\right)$ 

\item \hspce $8x^{9}y^3 - 64z^{6}$\\
$=8(x^{9}y^3 - 8z^{6}) $\\
$= 8[(x^{3} y)^3 - (2 z^{2})^3]$\\
$= 8 \left(x^{3} y - 2 z^{2}\right) \left(x^{6} y^{2} + 2 x^{3} y z^{2} + 4 z^{4}\right)$

\item \hspce $216x^{3} + 8y^9$\\
$=8(27x^{3} + y^9)$\\
$= 8[(3 x)^3 + (y^{3})^3]$\\
$= 8 \left(3 x + y^{3}\right) \left(9 x^{2} - 3 x y^{3} + y^{6}\right)$

\item \hspce $a^{3}b^6 - 64c^{9}d^{3}$\\
$= (a b^{2})^3 - ( 4 c^{3} d)^3$\\
$= \left(a b^{2} - 4 c^{3} d\right) \left(a^{2} b^{4} + 4 a b^{2} c^{3} d + 16 c^{6} d^{2}\right)$

\item \hspce $125m^{3} - 27n^{6}$\\
$= (5 m)^3 - (3 n^{2})^3$\\
$= \left(5 m - 3 n^{2}\right) \left(25 m^{2} + 15 m n^{2} + 9 n^{4}\right)$

\item \hspce $216a^{6} + 64b^9$\\
$= 8(27a^{6} + 8b^9)$\\
$= 8[(3 a^{2})^3 + (2 b^{3})^3]$\\
$= 8 \left(3 a^{2} + 2 b^{3}\right) \left(9 a^{4} - 6 a^{2} b^{3} + 4 b^{6}\right)$


% 
\end{enumerate}