\textbf{Problem Set}

\vspce

\begin{enumerate}[label = \arabic*. ]
\begin{multicols}{2}
%1
\item %\hspce $f(x) = (x-2)(x-1)(x-3)$\\
$a_n: +$, $n= 3 (odd)$, 
Case 1\\
$0 = (x-2)(x-1)(x-3)$\\
$x-2=0$ \\
$x=2$\\
$x-1=0$ \\
$x=1$\\
$x-3=0$ \\
$x=3$\\
$Roots=\{1, 2, 3\}$ 
%2
\item %\hspce $f(x) =x(x+1)^2$\\
$a_n: +$, $n=3(odd)$, 
Case 1\\
$0 = x(x+1)^2$\\
$x=0$ \\
$(x+1)^2=0$\\
$\sqrt{(x+1)^2}=\sqrt{0}$ \\
$x+1=0$\\
$x=-1$ of mult. 2\\
Roots=\{0, -1 of mult. 2\}
%3
\item %\hspce $f(x) =x(x-2)(x+1)(x+3)$\\
$a_n= +$, $n=4(even)$, 
Case 3\\
$0 = x(x-2)(x+1)(x+3)$\\
$x=0$\\
$x-2=0$ \\
$x=2$\\
$x+1=0$ \\
$x=-1$\\
$x+3=0$ \\
$x=-3$\\
$Roots=\{-3, -1, 0, 2\}$ \\
If $x=-2$:\\
$f(-2) =-2(-2-2)(-2+1)(-2+3)$\\
$f(-2) =-2(-4)(-1)(1)$\\
$f(-2) =-8$\\
$\therefore (-2, -8) $\\
If $x=1$:\\
$f(1) =1(1-2)(1+1)(1+3)$\\
$f(1) =1(-1)(2)(4)$\\
$f(1) =-8$\\
$\therefore (1, -8) $
%4
\item %\hspce $f(x) =(x+2)(x-1)(x-3)^2$\\
$a_n= +$, $n=4(even)$, 
Case 3\\
$0 = (x+2)(x-1)(x-3)^2$\\
$x+2=0$ \\
$x=-2$\\
$x-1=0$ \\
$x=1$\\
$(x-3)^2=0$ \\
$\sqrt{(x-3)^2}=\sqrt{0} $ \\
$x-3=0$ \\
$x=3$ of mult. 2\\
Roots=\{-2, 1, 3 of mult. 2\}


\end{multicols} 
\end{enumerate} 