\textbf{Problem Set}

\vspce

%Evaluate the following  rational expressions.

\begin{enumerate}[label = \arabic*. ]
%begin{multicols}{2}

\item \hspce% $\displaystyle \frac{1}{a^{-2}}(a+4),\hspce a=-8$
$\displaystyle \frac{1}{(-8)^{-2}}(-8+4)$\\
$=\displaystyle \frac{1}{\displaystyle \frac{1}{(-8)^{2}} }(-4)$\\
$=\displaystyle \frac{1}{\displaystyle \frac{1}{64} }(-4)$\\
$=(64)(-4)$\\
$=-256 $

\item \hspce% $(p^{3} - 5)^{-2},\hspce p=2$
$(2^{3} - 5)^{-2}$\\
$=\displaystyle \frac{1}{(2^{3} - 5)^{2}} $
$=\displaystyle \frac{1}{(8 - 5)^{2}} $\\
$=\displaystyle \frac{1}{3^{2}} $
$=\displaystyle\frac{1}{9} $

\item \hspce% $\displaystyle \frac{(x-2)^{-3}}{(x+1)^{-3}},\hspce x=4$
$\displaystyle \frac{(4-2)^{-3}}{(4+1)^{-3}}$\\
$=\displaystyle \frac{2^{-3}}{5^{-3}}$
$=\displaystyle \frac{\displaystyle \frac{1}{2^{3}} }{\displaystyle \frac{1}{5^{3}} }$\\
$=\displaystyle \frac{\displaystyle \frac{1}{8} }{\displaystyle \frac{1}{125} }$
$=\left( \displaystyle \frac{1}{8}\right) (125)$\\
$=\displaystyle\frac{125}{8} $\\

\item \hspce% $y^{-4}-y^{-3},\hspce y=3$
$3^{-4}-3^{-3}$\\
$=\displaystyle \frac{1}{3^{4}} -\displaystyle \frac{1}{3^{3}} $%\\
$=\displaystyle \frac{1}{81} -\displaystyle \frac{1}{27} $\\
$=\displaystyle - \frac{2}{81} $\\

\item \hspce% $\displaystyle \frac{(m-n)^{0}}{(m+n)^{-1}},\hspce m=2, n=3$
$\displaystyle \frac{(2-3)^{0}}{(2+3)^{-1}}$\\
$=\displaystyle \frac{1}{5^{-1}}$\\
$=\displaystyle \frac{1}{\displaystyle \frac{1}{5}} $\\
$=(1)(5)$\\
$=5 $


%end{multicols}
\end{enumerate}