\textbf{Problem Set}

\vspce
\begin{enumerate}
%begin{multicols}{2}

\item \hspce $4x^{2} - 49y^{2}$\\
$=(2 x )^2 - (7 y)^2$\\
$= \left(2 x - 7 y\right) \left(2 x + 7 y\right)$

\item \hspce $a^{2} - 100$\\
$=(a)^2 - (10)^2$\\
$= \left(a - 10\right) \left(a + 10\right)$

\item \hspce $y^{8} - 16z^{4}$\\
$=(y^{4})^2 - (4 z^{2})^2$\\
$= \left(y^{4} - 4 z^{2}\right) \left(y^{4} + 4 z^{2}\right)$\\
$= \left(y^{2} - 2 z\right) \left(y^{2} + 2 z\right) \left(y^{4} + 4 z^{2}\right)$

\item \hspce $y^{4} - 1$\\
$=(y^{2})^2 - (1)^2$\\
$= \left(y^{2} - 1\right) \left(y^{2} + 1\right)$\\
$= \left(y - 1\right) \left(y + 1\right) \left(y^{2} + 1\right)$

\item \hspce $25m^{2} - 9$\\
$=(5 m)^2 - (3)^2$\\
$= \left(5 m - 3\right) \left(5 m + 3\right)$

\item \hspce $144x^{6} - 100y^{4}$\\
$=4(36x^{6} - 25y^{4}) $\\
$=4[(6 x^{3})^2 - (5 y^{2})^2]$\\
$= 4 \left(6 x^{3} - 5 y^{2}\right) \left(6 x^{3} + 5 y^{2}\right)$

\item \hspce $a^{2}b^4 - 121$\\
$=(ab^2)^2 - (11)^2$\\
$= \left(a b^{2} - 11\right) \left(a b^{2} + 11\right)$

\item \hspce $x^{6}y^2 - 49z^{8}$\\
$=(x^{3} y)^2 - (7z^{4})^2$\\
$= \left(x^{3} y - 7 z^{4}\right) \left(x^{3} y + 7 z^{4}\right)$

\item \hspce $x^2y^{4} - 64$\\
$=(x y^{2})^2 - (8)^2$\\
$= \left(x y^{2} - 8\right) \left(x y^{2} + 8\right)$

\item \hspce $36m^{6} - 81$\\
$=9(4m^{6} - 9)$\\
$=9[(2 m^{3} )^2 - (3)^2]$\\
$= 9 \left(2 m^{3} - 3\right) \left(2 m^{3} + 3\right)$


%end{multicols} 
\end{enumerate}