\begin{center}
\textbf{Quiz \#2}
\end{center} 


\begin{enumerate}[label = \Alph*. ]
\begin{multicols}{2}

%A
\item \phantom{a}
\begin{enumerate}[label = \arabic*. ]
%1
\item %\#5 
$y^2-121$\\
$=(y)^2- (11)^2 $\\
$=\left(y - 11\right) \left(y + 11\right) $

%2
\item %\#15
$ x^2-\displaystyle \frac{1}{16} $\\
$=(x)^2- (\displaystyle \frac{1}{4})^2 $\\
$= (x-\displaystyle \frac{1}{4}) (x+\displaystyle \frac{1}{4}) $

%3
\item %\#17
$y^2-\displaystyle \frac{9}{25} $\\
$=(y)^2- (\displaystyle \frac{3}{5})^2 $\\
$=(y-\displaystyle \frac{3}{5}) (y+\displaystyle \frac{3}{5})  $

\end{enumerate}   


%B
\item \phantom{a}
\begin{enumerate}[label = \arabic*. ]
%1
\item %\#4
$ 144-16n^2$\\
$=16(9-n^2)$\\
$=16[(3)^2- (n)^2] $\\
$=16 \left( 3-n\right) \left( 3+n\right)$

%2
\item %\#5
$m^2n^2-196 $\\
$=(m n)^2- (14)^2 $\\
$= \left(m n - 14\right) \left(m n + 14\right)$

%3
\item %\#6
$ 169a^2-b^2c^2$\\
$=(13 a)^2- (b c)^2 $\\
$=\left(13 a - b c\right) \left(13 a + b c\right) $

\item %\#12
$\displaystyle \frac{1}{16} x^2- \displaystyle \frac{1}{25} y^2 $\\
$=(\displaystyle \frac{1}{4} x)^2- (\displaystyle \frac{1}{5} y)^2 $\\
$= \left(\displaystyle \frac{1}{4} x - \displaystyle \frac{1}{5} y\right) \left(\displaystyle \frac{1}{4} x + \displaystyle \frac{1}{5} y\right)$

\item %\#14
$ 144a^4-169b^4$\\
$=(12 a^{2})^2- (13 b^{2})^2 $\\
$= \left(12 a^{2} - 13 b^{2}\right) \left(12 a^{2} + 13 b^{2}\right)$

\item %\#15
$125x^2-180 $\\
$=5(25x^2-36) $\\
$=5[(5 x)^2- (6)^2 ]$\\
$=5 \left(5 x - 6\right) \left(5 x + 6\right)$

\item %\#18
$y^4-16 $\\
$=(y^2)^2- (4)^2 $\\
$=(y^2-4) (y^2+4) $\\
$=\left(y - 2\right) \left(y + 2\right) \left(y^{2} + 4\right)$

\item %\#19
$p^6-81 $\\
$=(p^{3})^2- (9)^2 $\\
$= \left(p^{3} - 9\right) \left(p^{3} + 9\right)$


\end{enumerate}   


\end{multicols} 
\end{enumerate}  