\begin{center}
\textbf{Solving Systems of Linear Equations by the Substitution Method}\\
\fbox{Total points = 61}
\end{center} 

%\begin{center}
%\vspace*{-2ex}
\scalebox{0.8}{
\noindent\begin{minipage}{\textwidth}
{

\begin{enumerate}[label = \arabic*. ]
\begin{multicols}{2}

\item $ 2x-y = 2$ \redcheck \\
$-1\left[-y =-2x+ 2\right] $ \redcheck \\
\fbox{$y =2x- 2 $} \redcheck \\

$6x+5y = 2 $ \redcheck \\
$6x+5(2x- 2) = 2 $ \redcheck \\
$6x+10x- 10 = 2 $ \redcheck \\
$16x = 2+ 10 $ \redcheck \\
$\dfrac{16x}{16}  = \dfrac{12}{16}  $ \redcheck \\
\fbox{$x = \dfrac{3}{4}  $} \redcheck \\

$ 2x-y = 2$ \redcheck \\
$ 2\left(\dfrac{3}{4}\right) -y = 2$ \redcheck \\
$ \dfrac{3}{2} -y = 2$ \redcheck \\
$  -y = -\dfrac{3}{2}+2$ \redcheck \\
$  -1 \left[ -y = \dfrac{1}{2}\right] $ \redcheck \\
\fbox{$ y = -\dfrac{1}{2} $} \redcheck \\

$\therefore$ Solution =\fbox{ $\left(\dfrac{3}{4}, -\dfrac{1}{2}\right) $ }\redcheck

\vspce 
\item $ x-3y  = 1$ \redcheck \\
\fbox{$ x  =3y+ 1$} \redcheck \\

$ -2x+6y  =  5$ \redcheck \\
$ -2(3y+ 1)+6y  =  5$ \redcheck \\
$ -6y-2+6y  =  5$ \redcheck \\
$ 0 =  5+2$ \redcheck \\
\fbox{$ 0 =  7$ }\redcheck \\

$\therefore$ Solution = \fbox{None }\redcheck

\vspce 
\item $ x-3y  = 1$ \redcheck \\
\fbox{$ x  =3y+ 1$} \redcheck \\

$ -2x+6y  =  -2$ \redcheck \\
$ -2(3y+ 1)+6y  =  -2$ \redcheck \\
$ -6y-2+6y  =  -2$ \redcheck \\
$ 0 =  -2+2$ \redcheck \\
\fbox{$ 0 =  0$ }\redcheck \\

$\therefore$ Solution = \fbox{None} \redcheck


\vspce 
\item $x+y  =  11 $ \redcheck \\
\fbox{$x  = -y +11 $} \redcheck \\

$ 3x-y  =  5$ \redcheck \\
$ 3(-y +11)-y  =  5$ \redcheck \\
$ -3y +33-y  =  5$ \redcheck \\
$ -4y   =  5-33$ \redcheck \\
$ \dfrac{-4y}{-4}    =  \dfrac{-28}{-4}$ \redcheck \\
\fbox{$ y =  7$} \redcheck \\

$x+y  =  11  $ \redcheck \\
$x+7  =  11  $ \redcheck \\
$x=  11 -7 $ \redcheck \\
\fbox{$x=  4 $} \redcheck \\

$\therefore$ Solution = \fbox{$\left(4, 7\right) $} \redcheck

\vspce 
\item $3x+2y  =  9 $ \redcheck \\
$\dfrac{2y}{2}   = -\dfrac{3x}{2}+ \dfrac{9}{2} $ \redcheck \\
\fbox{$y= -\dfrac{3x}{2}+ \dfrac{9}{2} $ }\redcheck \\

$ 3x =  4y -3$ \redcheck \\
$ 3x =  4\left( -\dfrac{3x}{2}+ \dfrac{9}{2}\right) -3$ \redcheck \\
$ 3x =  -6x+ 18 -3$ \redcheck \\
$ 3x +6x=  15$ \redcheck \\
$ \dfrac{9x}{9} = \dfrac{15}{9} $ \redcheck \\
\fbox{$ x = \dfrac{5}{3} $} \redcheck \\

$ 3x =  4y -3 $ \redcheck \\
$ 3\left( \dfrac{5}{3}\right) =  4y -3 $ \redcheck \\
$ 5 =  4y -3 $ \redcheck \\
$ 5 +3=  4y  $ \redcheck \\
$ \dfrac{8}{4} = \dfrac{4y}{4}   $ \redcheck \\
\fbox{$ y = 2$ }\redcheck \\

$\therefore$ Solution = \fbox{$\left(\dfrac{5}{3}, 2\right) $} \redcheck

\end{multicols} 
\end{enumerate}
}
\end{minipage}}
%\end{center} 
%