\textbf{Problem Set}

\vspce

A.   
\begin{enumerate}
\item \hspce $(2m - n + 3r)^{2} 
= (2m)^{2}+(- n)^{2}+(3r)^{2}+2(2m)(- n)+2(2m)(3r)\\+2(- n)(3r)\\
=4m^2+n^2+9r^2-4mn+12mr-6nr$ 
\item \hspce $(-4a + 2b - c)^{2}
= (-4a)^{2}+(2b)^{2}+(- c)^{2}+2(-4a)(2b)\\+2(-4a)(- c)+2(2b)(- c)\\
=16a^2+4b^2+c^2-16ab+8ac-4bc$
\item \hspce $(3h^{2} - 2i + k)^{2}
= (3h^{2})^{2}+(- 2i)^{2}+(k)^{2}+2(3h^{2})(- 2i)+2(3h^{2})(k)\\+2(- 2i)(k)\\
=9h^4+4i^2+k^2-12h^2i+6h^2k-4ik$
\item \hspce $(5x + 3y + 2z)(5x + 3y + 2z)
= (5x)^{2}+(3y)^{2}+(2z)^{2}+2(5x)(3y)\\+2(5x)(2z)+2(3y)(2z)\\
=25x^2+9y^2+4z^2+30xy+20xz+12yz$
\item \hspce $(2m - 4n^{3} - 2r)^{2}
= (2m)^{2}+(- 4n^{3})^{2}+(- 2r)^{2}+2(2m)(- 4n^{3})+2(2m)(- 2r)+2(- 4n^{3})(- 2r)\\
=4m^2+16n^6+4r^2-16mn^3-8mr+16n^3r$
\end{enumerate}

B.  
\begin{enumerate}[label = \arabic*. ]
%%begin{multicols}{2}
%1
\item \hspce $(2x - y + 3z)^{2}\\
= (2x)^{2}+(- y)^{2}+(3z)^{2}+2(2x)(- y)+2(2x)(3z)+2(- y)(3z) \\
= 4 x^{2} + y^{2} + 9z^2  - 4 x y + 12 x z  - 6yz  $\\
Missing terms = $9z^2$, $6yz$
% 4 x^{2} + y^{2} + 9 z^{2} - 4 x y + 12 x z  - 6 y z 

%2
\item \hspce $(3x + 2y^{2} - z)^{2}\\
= (3x)^{2}+(2y^{2})^{2}+(z)^{2}+2(3x)(2y^{2})+2(3x)(z)+2(2y^{2})(z) \\
= 9 x^{2} + 4 y^{4} + z^{2} + 12xy^2  - 6xz   - 4 y^{2} z$\\
Missing terms = $12xy^2 $, $6xz$
% 9 x^{2} + 4 y^{4} + z^{2} + 12 x y^{2} - 6 x z  - 4 y^{2} z 
%3
\item \hspce $(-x^{2} - 3y^{3} + 2z)^{2}
= (-x^{2})^{2}+(- 3y^{3})^{2}+(2z)^{2}+2(-x^{2})(- 3y^{3})+2(-x^{2})(2z)+2(- 3y^{3})(2z) \\
= x^{4} + 9 y^{6} + 4 z^{2} + 6 x^{2} y^{3}  - 4 x^{2} z - 12 y^{3} z  $\\
% x^{4} + 9 y^{6} + 4 z^{2} + 6 x^{2} y^{3} - 4 x^{2} z - 12 y^{3} z 
Missing terms = $6 x^{2} y^{3} $, $12 y^{3} z $
%4
\item \hspce $(-tx^{2} + 2y^{2} - 3z)^{2}
= (-tx^{2})^{2}+(2y^{2})^{2}+(- 3z)^{2}+2(-tx^{2})(2y^{2})+2(-tx^{2})(- 3z)+2(2y^{2})(- 3z) \\
= t^{2} x^{4} + 4 y^{4}  + 9 z^{2} - 4 t x^{2} y^{2}  + 6 t x^{2} z  - 12 y^{2} z $\\
Missing terms = $4 y^{4}$, $4 t x^{2} y^{2}$
% t^{2} x^{4} + 4 y^{4} + 9 z^{2} - 4 t x^{2} y^{2} + 6 t x^{2} z  - 12 y^{2} z 

%5 
\item \hspce $(-4t + 2x^{2}y^{3} - 3z^{3})^{2}\\
= (-4t)^{2}+(2x^{2}y^{3})^{2}+(- 3z^{3})^{2}+2(-4t)(2x^{2}y^{3})+2(-4t)(- 3z^{3})+2(2x^{2}y^{3})(- 3z^{3}) \\
= 16 t^{2} + 4 x^{4} y^{6} + 9 z^{6} - 16 t x^{2} y^{3}  + 24 t z^{3}  - 12 x^{2} y^{3} z^{3}  $\\
Missing terms = $16 t x^{2} y^{3}$, $12 x^{2} y^{3} z^{3}$


% 16 t^{2} + 4 x^{4} y^{6} + 9 z^{6} - 16 t x^{2} y^{3} + 24 t z^{3}  - 12 x^{2} y^{3} z^{3} 
%%end{multicols} 
\end{enumerate}  