\textbf{Problem Set}

\vspce

A.  
\begin{enumerate}
%%begin{multicols}{2}

\item \hspce $(2m + 3r)^{3}$\\
$=(2m)^{3}+3(2m)^{2}(3r)+3(2m)(3r)^{2}+(3r)^{3}$\\
$=8m^3+9r(4m^2)+6m(9r^2)+27r^3$\\
$=8m^3+36m^2r+54mr^2+27r^3$

\item \hspce $(-4a - c)^{3}$\\
$=(-4a)^{3}+3(-4a)^{2}(- c)+3(-4a)(- c)^{2}+(- c)^{3}$\\
$=-64a^{3}-3c(16a^{2})-12a(c^{2})- c^{3}$\\
$=-64a^{3}-48a^{2}c-12ac^{2}- c^{3}$

\item \hspce $(3h^{2} - 2i)^{3}$\\
$=(3h^{2})^{3}+3(3h^{2})^{2}(- 2i)+3(3h^{2})(- 2i)^{2}+(- 2i)^{3}$\\
$=27h^{6}-6i(9h^{4})+9h^{2}(4i^{2}) -8i^{3}$\\
$=27h^{6}-54h^{4}i+36h^{2}i^{2} -8i^{3}$

\item \hspce $(5x + 3y)^{3}$\\
$=(5x)^{3}+3(5x)^{2}(3y)+3(5x)(3y)^{2}+(3y)^{3}$\\
$= 125x^{3} + 9y(25x^{2}) + 15x(9y^{2}) + 27y^{3}$\\
$= 125x^{3} + 225x^{2}y + 135xy^{2} + 27y^{3}$

\item \hspce $(2m - 4n^{3})^{3}$\\
$=(2m)^{3} + 3(2m)^{2}(-4n^{3}) + 3(2m)(-4n^{3})^{2} + (-4n^{3})^{3}$\\
$=8m^{3} - 12n^{3}(4m^{2}) + 6m(16n^{6}) - 64n^{9}$\\
$=8m^{3} - 48m^{2}n^{3} + 96mn^{6} - 64n^{9}$

%%end{multicols} 
\end{enumerate}

B. %Fill in the blanks. 
\begin{enumerate}[label = \arabic*. ]
%%begin{multicols}{2}
%1
\item \hspce %$(2x - y)^{3}$\\
$=(2x)^{3} + 3(2x)^{2}(- y) + 3(2x)(- y)^{2} + (- y)^{3}$\\
$=8x^{3} - 3y(4x^{2}) + 6x(y^{2}) - y^{3}$\\
% =  8 x^{3} - \blank  + \blank  - y^{3}$
$= 8 x^{3} - 12 x^{2} y + 6 x y^{2} - y^{3}$\\
Missing terms = $12 x^{2} y$, $6 x y^{2}$

%2
\item \hspce %$(3x + z^3)^{3}$\\
$=(3x)^{3} + 3(3x)^{2}(z^3) + 3(3x)(z^3)^{2} + (z^3)^{3}$\\
$=27x^{3} + 3z^3(9x^{2}) + 9x(z^6) + z^9$\\
% = \blank  + \blank  + 9 x z^{6} + z^{9}$
$= 27 x^{3} + 27 x^{2} z^{3} + 9 x z^{6} + z^{9}d$\\
Missing terms = $27 x^{3} $, $27 x^{2} z^{3}$

%3
\item \hspce %$(-2t^2 - y^3)^{3}$\\
$=(-2t^2)^{3} + 3(-2t^2)^{2}(y^3) + 3(-2t^2)(y^3)^{2} + (y^3)^{3}$\\
$=-8t^6 + 3y^3(4t^4)  - 6t^2(y^6) + y^9$\\
% = - 8 t^{6} - \blank  - \blank  - y^{9} $
$= - 8 t^{6} - 12 t^{4} y^{3} - 6 t^{2} y^{6} - y^{9}$\\
Missing terms = $12 t^{4} y^{3}$, $6 t^{2} y^{6}$

%4
\item \hspce %$(-3xy^2 + z^2 )^{3}$\\
$=(-3xy^2)^{3} + 3(-3xy^2)^{2}(z^2) + 3(-3xy^2)(z^2)^{2} + (z^2)^{3}$\\
$=-27x^3y^6 + 3z^2(9x^2y^4)  -9xy^2(z^4) + z^6$\\
% = - 27 x^{3} y^{6} + \blank  - \blank  + z^{6}$
$= - 27 x^{3} y^{6} + 27 x^{2} y^{4} z^{2} - 9 x y^{2} z^{4} + z^{6}$\\
Missing terms = $27 x^{2} y^{4} z^{2}$, $9 x y^{2} z^{4}$

%5 
\item \hspce %$(3x^3y^2 - 2z^2)^{3}$\\
$=(3x^3y^2)^{3} + 3(3x^3y^2)^{2}(-2z^2) + 3(3x^3y^2)(-2z^2)^{2} \\+ (-2z^2)^{3}$\\
$=27x^9y^6 - 6z^2(9x^6y^4) + 9x^3y^2(4z^4) - 8z^6$\\
% $= \blank  - \blank  + 36 x^{3} y^{2} z^{4} - 8 z^{6}$
$=27 x^{9} y^{6} - 54 x^{6} y^{4} z^{2} + 36 x^{3} y^{2} z^{4} - 8 z^{6}$\\
Missing terms = $27 x^{9} y^{6}$, $54 x^{6} y^{4} z^{2}$\\
%%end{multicols} 
\end{enumerate}  