B. Fill in the blanks. 
\begin{enumerate}[label = \arabic*. ]
%%begin{multicols}{2}
%1
\item \hspce $(x - 3y)^{3} = x^{3} - \blank  + 27 x y^{2} - \blank $
% x^{3} - 9 x^{2} y + 27 x y^{2} - 27 y^{3}
%2
\item \hspce $(2x + z^2)^{3} = 8 x^{3} + \blank  + \blank  + z^{6}$
% 8 x^{3} + 12 x^{2} z^{2} + 6 x z^{4} + z^{6}
%3
\item \hspce $(-3t^2 - 2y^3)^{3} = - 27 t^{6} - \blank  - 36 t^{2} y^{6} - \blank  $
% - 27 t^{6} - 54 t^{4} y^{3} - 36 t^{2} y^{6} - 8 y^{9}
%4
\item \hspce $(-xy^2 + 3z^2 )^{3} = \blank  + 9 x^{2} y^{4} z^{2} - \blank  + 27 z^{6}$
% - x^{3} y^{6} + 9 x^{2} y^{4} z^{2} - 27 x y^{2} z^{4} + 27 z^{6}
%5 
\item \hspce $(x^2y^3 - 2z^3)^{3} = x^{6} y^{9} - \blank  + \blank  - 8 z^{9}$
% x^{6} y^{9} - 6 x^{4} y^{6} z^{3} + 12 x^{2} y^{3} z^{6} - 8 z^{9}
%%end{multicols} 
\end{enumerate}  